proof/correctness/Properties.ec
@@ -17,6 +17,8 @@ require import Termination Repr.
 require import BitEncoding.
 (*---*) import BitChunking.
 
+(*** sizes ***)
+
 lemma size_prf : hoare[Hash.prf : true ==> size res = n]
     by proc; seq 2 : (#pre); auto => />; smt(size_hash).
 
@@ -41,3 +43,51 @@ qed.
 
 lemma ssize_chain : phoare[Chain.chain : size X = n ==> size res.`1 = n] = 1%r 
     by conseq chain_ll size_chain; auto => />. 
+
+
+(*** Base W Bounds ***)
+
+lemma base_w_size (l : int) :
+    0 < l => 
+    hoare [ BaseW.base_w : arg.`2 = l ==> size res = l].
+proof.
+move => ?. 
+proc.
+seq 6 : (#post); first by auto => />; rewrite size_nseq /#. 
+while (#pre); last by skip.
+if; auto => /> *; by rewrite size_put. 
+qed.
+
+lemma base_w_bounds (t : W8.t list) (il ol : int):
+    0 < il /\ 0 < ol /\ size t = il =>
+    hoare [ 
+        BaseW.base_w : 
+        arg = (t, ol)
+        ==> (*       (forall (k : int), 0 <= k < l => 0 <= nth witness res k < w) *)
+        forall (x : int), x \in res => 0 <= x < w
+      ].
+proof.
+move => [#] ???.
+conseq (:_ ==> (forall (k : int), 0 <= k < size res => 0 <= nth witness res k < w)); first by auto => /> *; smt(@List). 
+proc.
+auto.
+seq 6 : (#pre /\ out = 0 /\ size base_w = ol /\ consumed = 0); first by auto => /> *; rewrite size_nseq /#.
+while (
+  0 < outlen /\
+  size base_w = ol /\
+  out = consumed /\
+  0 <= consumed <= outlen /\
+  (forall (k : int), 0 <= k < consumed => 0 <= nth witness base_w k < w)
+); last first. 
+    + auto => /> &hr *;  smt(). 
+if.
+admit.
+auto => /> &hr *. 
+rewrite size_put. do split; 1,2:smt(). 
+move => k Hk0 Hk1.
+split. 
+    + rewrite nth_put. split; [smt() |]. admit. case (consumed{hr} = k); admit.
+    + rewrite nth_put. split; [smt() |]. admit. case (consumed{hr} = k).
+       - move => *. admit.
+    + smt(@List). 
+qed.
